test.fst
@@ -1,24 +1,55 @@
 module Test
 
 open FStar
-open FStar.ST
-open FStar.Mul
-open FStar.UInt
 open FStar.Buffer
 open FStar.Int.Cast
+open FStar.Mul
 
 module U8 = FStar.UInt8
 module U32 = FStar.UInt32
 
-#reset-options "--initial_fuel 1 --max_fuel 1"
+//#reset-options "--initial_fuel 1 --max_fuel 1"
+#reset-options "--max_fuel 1 --z3rlimit 100"
+
+
+private (* HACL* -> FStar.Endianness *)
+let rec big_endian (b:FStar.Seq.seq U8.t) : Tot nat (decreases (FStar.Seq.length b)) =
+  let open FStar.Seq in
+  if length b = 0 then 0
+  else
+    U8.v (last b) + pow2 8 * big_endian (slice b 0 (length b - 1))
+
+private
+val big_endian_zero: len:nat{len <= 4} -> Lemma
+  (ensures (big_endian (Seq.create len 0uy) == 0))
+  (decreases (len))
+let rec big_endian_zero len =
+  let open FStar.Seq in
+  if len = 0 then ()
+  else (
+    let nlen = len - 1 in
+    lemma_eq_intro (slice (create len 0uy) 0 nlen) (create nlen 0uy);
+    //assert (big_endian (create len 0uy) == 0 + pow2 8 * big_endian (slice (create len 0uy) 0 (len - 1)));
+    big_endian_zero nlen
+  )
+
+private
+val big_endian_single: n:U8.t -> Lemma
+  (ensures (big_endian (Seq.create 1 n) == U8.v n))
+let big_endian_single n =
+  let open FStar.Seq in
+  let s = (create 1 n) in
+  assert (big_endian s == U8.v (index s 0) + pow2 8 * big_endian (slice s 0 0))
+
+
 
 
 val read_length :
   buf:buffer U8.t ->
-  len:U32.t{U32.v len < 5} ->
-  Stack (r:U32.t{U32.v r < pow2 (8 * U32.v len)})
+  len:U32.t{U32.v len <= 4} ->
+  ST (r:U32.t{U32.v r < pow2 (8 * U32.v len)})
   (requires (fun h -> live h buf /\ U32.v len == length buf))
-  (ensures (fun h0 _ h1 -> h0 == h1 /\ live h1 buf))
+  (ensures (fun h0 r h1 -> h0 == h1 /\ live h1 buf /\ U32.v r == big_endian (as_seq h0 buf)))
   (decreases (length buf))
 
 let rec read_length buf len =
@@ -29,58 +60,138 @@ let rec read_length buf len =
     let bi = index buf len in
     let lo = uint8_to_uint32 bi in
     Math.Lemmas.pow2_plus 8 24;
+    // TODO assert Buffer.sub
     let hi = read_length (Buffer.sub buf 0ul len) len in
     assert (U32.v hi < pow2 (8 * (U32.v len)));
     let hi' = hi <<^ 8ul in
+    assert (hi = 0ul ==> hi' = 0ul);
     let res = hi' |^ lo in
     UInt.logor_disjoint #32 (v hi') (v lo) 8;
     assert (v res == pow2 8 * (v hi) + (v lo));
+    assert (hi' = 0ul ==> res = lo);
+    assert (lo = 0ul ==> res = hi');
+    assert (hi' = 0ul /\ lo = 0ul ==> res = 0ul);
     res
   )
+
+(*
+private // TODO len <= 4
+val test_parse_long_zero : len:U32.t{U32.v len < 2} -> St unit
+
+let rec test_parse_long_zero len = match (U32.v len) with
+  | 0 -> ()
+  | 1 -> (
+      push_frame ();
+      let sdata = Seq.create (U32.v len - 1) 0uy in
+      //let data = create 0uy U32.(len -^ 1ul) in
+      let data = of_seq sdata U32.(len -^ 1ul) in
+      assert (length data = 0);
+      assert (read_length data 0ul = 0ul);
+      //Seq.lemma_index_create (U32.v len - 1) 0uy (U32.v len - 2);
+      let h = ST.get() in
+      Seq.lemma_eq_intro (as_seq h data) (Seq.create (U32.v len - 1) 0uy);
+      assert (read_length data U32.(len -^ 1ul) = 0ul);
+      pop_frame ()
+
+      //push_frame ();
+      //test_parse_long_zero U32.(len -^ 1ul);
+      //let data = create 0uy len in
+      //let h = ST.get() in
+      //Seq.lemma_eq_intro (as_seq h data) (Seq.create (U32.v len) 0uy);
+      //assert (read_length data len = 0ul);
+      //pop_frame ()
+    )
+  *)
+
+  //push_frame ();
+  //let data = create 0uy len in
+  //let h = ST.get() in
+  //Seq.lemma_index_create 1 0x80uy 0;
+  //Seq.lemma_eq_intro (as_seq h data) (Seq.create (U32.v len) 0uy);
+  //assert (get h data 0 = 0uy);
+  //let out_len = create 1ul 1ul in
+  //Seq.lemma_index_create 1 0ul (U32.v len);
+  //let h = ST.get() in
+  //Seq.lemma_eq_intro (as_seq h out_len) (Seq.create 1 1ul);
+  //assert (read_length data len = 0ul);
+  //let h = ST.get() in
+  //assert (not success && get h out_len 0 = 0ul);
+  //assert (get h out_len 0 = 0ul);
+  //Seq.lemma_eq_intro (as_seq h out_len) (Seq.create 1 0ul);
+  //pop_frame ()
 
 
 val parse_len :
   buf:buffer U8.t ->
   len:U32.t{U32.v len = length buf /\ U32.v len > 0} ->
   out_len:buffer U32.t{length out_len = 1} ->
-  Stack bool
-  (requires (fun h -> live h buf /\ live h out_len /\ (get h out_len 0) = 0ul))
-  (ensures (fun h0 r h1 -> live h1 buf /\ live h1 out_len /\ (r \/ (get h1 out_len 0) = 0ul)))
+  ST bool
+  (requires (fun h -> live h buf /\ live h out_len))
+  (ensures (fun h0 r h1 -> live h1 buf /\ live h1 out_len /\
+            (r \/ (get h1 out_len 0) = 0ul)))
 
 let parse_len buf len out_len =
   let b0 = index buf 0ul in
   // Length bits.
-  let ilen = U8.(b0 &^ 127uy) in
+  let ilen = U8.(b0 &^ 0x7fuy) in
   UInt.logand_mask (U8.v b0) 7;
-  assert (U8.v ilen < 128);
+  assert (U8.v ilen < 0x80);
   // Length form.
   let is_short_form = (b0 = ilen) in
-  assert (is_short_form ==> not (nth (U8.v b0) 0));
+  assert (is_short_form ==> not (UInt.nth (U8.v b0) 0));
   let ilen = uint8_to_uint32 ilen in
 
   // Handle short form first.
   let res = if is_short_form then
     ilen
+  // Reject long form with zero bytes.
+  else if U32.(ilen =^ 0ul) then
+    0ul
   // Accept 4 bytes max. for long form.
   else if U32.(ilen >^ 4ul) then
     0ul
   // Check that we have enough bytes.
   else if U32.(len <=^ ilen) then
     0ul
-  // Reject long form with zero bytes.
-  else if ilen = 0ul then
-    0ul
   // Parse long form.
   else (
     assert (not is_short_form);
     assert (length buf > U32.v ilen);
     assert (U32.v ilen > 0 && U32.v ilen < 5);
-    read_length (Buffer.sub buf 1ul ilen) ilen
+    let lbytes = Buffer.sub buf 1ul ilen in
+    let h = ST.get() in // TODO
+    Seq.lemma_eq_intro (as_seq h lbytes) (Seq.slice (as_seq h buf) 1 (U32.v ilen + 1));
+    read_length lbytes ilen
   ) in
 
+  // Write the result. (TODO write without temp var?)
   out_len.(0ul) <- res;
+
   // If we picked a result > 0, success.
   // If the result is 0 because ilen is 0, only accept the short form.
-  U32.(res >^ 0ul) || (ilen = 0ul && is_short_form)
+  let success = U32.(res >^ 0ul) || (ilen = 0ul && is_short_form) in
 
-// TODO tests
+  // Short form is easy to parse.
+  assert (U8.(b0 <^ 0x80uy) ==> res = (uint8_to_uint32 b0) /\ success);
+  // TODO
+  //assert (U8.(b0 >^ 0x80uy /\ b0 <^ 0x85uy) /\
+          //(U32.v len > (U8.v b0) - 0x80) ==> U32.(res >=^ 0ul) /\ success);
+
+  let h = ST.get() in
+  // Fail when given a zero length in long form.
+  assert (b0 = 0x80uy ==> res = 0ul /\ not success);
+  // We can't parse long form with more than 4 bytes.
+  assert (U8.(b0 >^ 0x84uy) ==> res = 0ul /\ not success);
+  // The long form must have enough length bytes.
+  assert (U8.(b0 >^ 0x80uy /\ b0 <^ 0x85uy) /\
+          (U32.v len <= (U8.v b0) - 0x80) ==> res = 0ul /\ not success);
+  // The long form must not be all zero bytes. TODO
+  //Seq.lemma_len_slice (as_seq h buf) 1 ((U8.v b0) - 0x80 + 1);
+  //Seq.lemma_index_create ((U8.v b0) - 0x80) 0uy ((U8.v b0) - 0x80 - 1);
+  //assert (U8.(b0 >^ 0x80uy /\ b0 <^ 0x85uy) /\
+          //(U32.v len > (U8.v b0) - 0x80) /\
+          //(Seq.equal (Seq.slice (as_seq h buf) 1 ((U8.v b0) - 0x80 + 1)) (Seq.create ((U8.v b0) - 0x80) 0uy)) ==> res = 0ul /\ not success);
+
+  // TODO check long form with starting zero bytes
+
+  success
